acceptor.dfy
@@ -1,0 +1,57 @@
+class Acceptor<T(==)>
+{
+  var promise:  int;
+  var accepted: Accepted<T>;
+
+  constructor ()
+    modifies this;
+  { accepted := new Accepted(); }
+
+  method Prepare(round: int, value: T) returns (acp: Accepted<T>)
+	requires valid();
+    modifies this;
+	ensures valid() && promise >= round;
+  {
+    // is the round at least as new as our promise
+	// and we have not already accepted it?
+    if round >= promise && round != accepted.round {
+      promise := round;
+	  assert promise > accepted.round;
+	  // TODO: store state?
+      return accepted;
+    }
+	return null;
+  }
+
+  method Accept(round: int, value: T) returns (acp: Accepted<T>)
+	requires valid();
+    modifies this, accepted;
+	ensures valid() && promise >= round;
+  {
+    // is the round at least as new as our promise?
+    if round >= promise {
+      promise       := round;
+      accepted.round := round;
+      accepted.value   := value;
+	  // TODO: store state
+	  return accepted;
+    }
+	return null;
+  }
+
+  method Get() returns (rnd: int, acp: int, val: T)
+    requires valid();
+  { return promise, accepted.round, accepted.value; }
+
+  predicate valid()
+    reads this, accepted;
+  { accepted != null && promise >= accepted.round }
+}
+
+class Accepted<T(==)>
+{
+  var round: int;
+  var value: T;
+
+  constructor () {}
+}
